AP/AP/Determinacy.lean
@@ -75,7 +75,7 @@ sys.tr sd (st.d.f sd) = some sa' → p sa') : sa₀.aWins st ∧ p sa₀ := by
   have ha : AState sa
   · replace ih := congrArg (·.1) ih; subst ih; infer_instance
   simp [ih]
-  specialize h (sys.reachable_of_simulate_eq ih) hp
+  specialize h (sys.reachable_of_simulate ih) hp
   obtain ⟨sd, h₁, h₂⟩ := h
   simp [h₁]
   have hd := DState.of_tr h₁
@@ -119,6 +119,7 @@ def aStratChoose (p : State → Prop) : AStrat :=
 theorem wf_aStratChoose {p} : (aStratChoose p).WF := by
   unfold aStratChoose; infer_instance
 
+@[simp, grind ·]
 instance {p} : (aStratChoose p).WF := wf_aStratChoose
 
 theorem AState.aHws_of_ind_two' {sa₀ : State} [ha₀ : AState sa₀] {p : State → Prop}
@@ -147,6 +148,7 @@ theorem AState.aHws_of_ind_two {sa₀ : State} [ha₀ : AState sa₀] {p : State
 sys.tr sd pd = some sa' → p sa') : sa₀.aHws :=
   ha₀.aHws_of_ind_two' h₁ h₂ |>.1
 
+@[simp, grind ·]
 instance {s} [hs : sys.WF s] : sys.Tree s := by
   rw [System.tree_iff_full_trs]
   use hs; intro ts₁ ts₂ s' h₁ h₂
@@ -274,7 +276,8 @@ def dStratOfDWins (sa : State) : DStrat := .mk # λ sd => do
       ∀ (a : AStrat), a.WF → sa'.dWins ⟨a, d⟩
     return d.f sd
 
-instance {sa} : (dStratOfDWins sa).WF := by unfold dStratOfDWins; infer_instance
+instance {sa} : (dStratOfDWins sa).WF := by
+  unfold dStratOfDWins; infer_instance
 
 def AStrat.set (a : AStrat) (s : State) (p : PointZ) : AStrat := ⟨fn_set s p a.f⟩
 def DStrat.set (d : DStrat) (s : State) (p : PointZ) : DStrat := ⟨fn_set s p d.f⟩
@@ -312,7 +315,7 @@ sys.simulate st₂.f s k = (sd, 0) → sys.hasTr sd → st₁.d.f sd = st₂.d.f
 sys.simulate st₁.f s n = sys.simulate st₂.f s n := by
   apply System.simulate_congr
   intro k hk s₁ h₄ h₅ h₆
-  have h₇ := System.wf_of_reachable # System.reachable_of_simulate_eq h₄
+  have h₇ := System.wf_of_reachable # System.reachable_of_simulate h₄
   replace h₇ := s₁.aState_or_dState
   rcases h₇ with ha | hd <;> simp
   · apply h₁ <;> assumption
@@ -370,14 +373,14 @@ theorem AState.aHws_of_not_dHws {sa} [ha : AState sa] (h : ¬sa.dHws) : sa.aHws 
     replace H₄ := H₄.2 (by rfl) h₂
     rintro rfl
     apply H₄
-    exact System.reachable_of_simulate_eq H₂
+    exact System.reachable_of_simulate H₂
   apply simulate_congr <;> simp only [implies_true]
   intro k hk b hb H₁ H₂ H₃
   replace H₃ : b.getMoveAt sa = some pa
   · apply getMoveAt_eq_some_of_tr_and_reachable h₁
     trans sa'
     · exact System.reachable_of_tr h₂
-    · exact System.reachable_of_simulate_eq H₁
+    · exact System.reachable_of_simulate H₁
   simp [dStratOfDWins, mk_strat_fn, H₃, h₁]; clear H₃
   rw [choose?_eq_of_exi, Hpd]; rotate_left; exact h
   simp
@@ -397,7 +400,8 @@ def aStratOfAHws (sd : State) : AStrat := .mk # λ sa => do
     ∀ (d : DStrat), d.WF → sa'.aWins ⟨a, d⟩
   return a.f sa
 
-instance {s} : (aStratOfAHws s).WF := by unfold aStratOfAHws; infer_instance
+instance {s} : (aStratOfAHws s).WF := by
+  unfold aStratOfAHws; infer_instance
 
 theorem AState.dHws_of_tr' {sd sa pd} [hd : DState sd]
 (h₁ : sys.tr sd pd = some sa) (h₂ : sa.dHws) : sd.dHws := by
@@ -425,7 +429,7 @@ theorem AState.dHws_of_tr' {sd sa pd} [hd : DState sd]
   have H₆ : sys.Acyclic b := inferInstance
   replace H₆ := H₆.2 (by rfl) h₁
   exfalso; apply H₆
-  exact System.reachable_of_simulate_eq H₂
+  exact System.reachable_of_simulate H₂
 
 theorem DState.aHws_of_tr' {sa sd pa} [ha : AState sa]
 (h₁ : sys.tr sa pa = some sd) (h₂ : sd.aHws) : sa.aHws := by
@@ -452,7 +456,7 @@ theorem DState.aHws_of_tr' {sa sd pa} [ha : AState sa]
   have H₆ : sys.Acyclic b := inferInstance
   replace H₆ := H₆.2 (by rfl) h₁
   exfalso; apply H₆
-  exact System.reachable_of_simulate_eq H₂
+  exact System.reachable_of_simulate H₂
 
 theorem State.aHws_of_not_dHws {s : State} [hs : sys.WF s]
 (h : ¬s.dHws) : s.aHws := by
@@ -482,7 +486,7 @@ theorem State.aHws_of_not_dHws {s : State} [hs : sys.WF s]
   intro k hk b H₅ H₂ H₃ H₄
   have H₆ : b.getMoveAt sd = some (d.f sd)
   · apply getMoveAt_eq_some_of_tr_and_reachable h₁
-    exact System.reachable_of_simulate_eq H₂
+    exact System.reachable_of_simulate H₂
   simp [aStratOfAHws, mk_strat_fn, H₆, h₁]
   rw [choose?_eq_of_exi, h₂]; rotate_left; exact h
   simp [h₃.validTr H₄]
@@ -729,7 +733,7 @@ theorem length_hist_sub_eq_of_simulate {s₀ s n f} [hs : sys.WF s₀]
   rw [Nat.sub_add_cancel]
   have h₂ : s'.hist.length ≤ s.hist.length
   · apply length_hist_le_of_reachable
-    exact System.reachable_of_simulate_eq h
+    exact System.reachable_of_simulate h
   have h₃ : s₀.hist.length < s'.hist.length
   · exact State.length_hist_lt_of_tr h₁
   omega
@@ -845,7 +849,7 @@ theorem State.simulate_set_a_eq_of_length_hist_lt {s s₁ p₁ n} {a : AStrat} {
 sys.simulate (Strat.mk (a.set s₁ p₁) d).f s n = sys.simulate (Strat.mk a d).f s n := by
   have h₃ := a.wf_set_of_validTr h₁; apply simulate_congr <;> simp
   intro k hk sa hsa h₄ h₅ h₆; rw [fn_set_eq_of_ne]; rintro rfl; contrapose! h₂
-  exact length_hist_le_of_reachable # System.reachable_of_simulate_eq h₅
+  exact length_hist_le_of_reachable # System.reachable_of_simulate h₅
 
 theorem State.simulate_set_d_eq_of_length_hist_lt {s s₁ p₁ n} {a : AStrat} {d : DStrat}
 [hs : sys.WF s] [hs₁ : sys.WF s₁] [ha : a.WF] [hd : d.WF]
@@ -853,7 +857,7 @@ theorem State.simulate_set_d_eq_of_length_hist_lt {s s₁ p₁ n} {a : AStrat} {
 sys.simulate (Strat.mk a (d.set s₁ p₁)).f s n = sys.simulate (Strat.mk a d).f s n := by
   have h₃ := d.wf_set_of_validTr h₁; apply simulate_congr <;> simp
   intro k hk sa hsa h₄ h₅ h₆; rw [fn_set_eq_of_ne]; rintro rfl; contrapose! h₂
-  exact length_hist_le_of_reachable # System.reachable_of_simulate_eq h₅
+  exact length_hist_le_of_reachable # System.reachable_of_simulate h₅
 
 theorem State.simulate_set_a_eq_of_le_length_hist_sub {s s₁ p₁ n} {a : AStrat} {d : DStrat}
 [hs : sys.WF s] [hs₁ : sys.WF s₁] [ha : a.WF] [hd : d.WF]
